src/Util/Tactics/Beta1.v
@@ -1,0 +1,6 @@
+Require Export Crypto.Util.Notations.
+
+Ltac beta1 x :=
+  lazymatch x with
+  | (fun a => ?f) ?b => constr:(subst_let a := b in f)
+  end.
