src/Util/Tactics/GeneralizeOverHoles.v
@@ -1,0 +1,8 @@
+Require Export Crypto.Util.FixCoqMistakes.
+Require Import Crypto.Util.Tactics.Zeta1.
+Require Import Coq.ssr.ssreflect.
+
+Ltac generalize_over_holes tac :=
+  zeta1 (ltac:(let H := fresh in
+               (pose H := ltac:(let v := tac () in refine v));
+               exact H)).
